2023/P01.lean
@@ -1,4 +1,52 @@
 import Lib
 
-def main : IO Unit := do
-  IO.println "ready!"
+private def loop (parse : List Char → Option ℕ) : List Char → List ℕ
+| cs@(_ :: cs') => match parse cs with
+                   | .some d => d :: loop parse cs'
+                   | .none => loop parse cs'
+| [] => []
+
+def List.parse_digits := loop $
+  λ | '1' :: _ => .some 1
+    | '2' :: _ => .some 2
+    | '3' :: _ => .some 3
+    | '4' :: _ => .some 4
+    | '5' :: _ => .some 5
+    | '6' :: _ => .some 6
+    | '7' :: _ => .some 7
+    | '8' :: _ => .some 8
+    | '9' :: _ => .some 9
+    | _ => .none
+
+def List.parse_digits' := loop $
+  λ | '1' :: _
+    | 'o' :: 'n' :: 'e' :: _               => .some 1
+    | '2' :: _
+    | 't' :: 'w' :: 'o' :: _               => .some 2
+    | '3' :: _
+    | 't' :: 'h' :: 'r' :: 'e' :: 'e' :: _ => .some 3
+    | '4' :: _
+    | 'f' :: 'o' :: 'u' :: 'r' :: _        => .some 4
+    | '5' :: _
+    | 'f' :: 'i' :: 'v' :: 'e' :: _        => .some 5
+    | '6' :: _
+    | 's' :: 'i' :: 'x' :: _               => .some 6
+    | '7' :: _
+    | 's' :: 'e' :: 'v' :: 'e' :: 'n' :: _ => .some 7
+    | '8' :: _
+    | 'e' :: 'i' :: 'g' :: 'h' :: 't' :: _ => .some 8
+    | '9' :: _
+    | 'n' :: 'i' :: 'n' :: 'e' :: _        => .some 9
+    | _ => .none
+
+def sum_by (parse_digits : List Char → List ℕ) : IO Unit := do
+  let lines ← (← IO.getStdin).lines
+  let nums := lines.map (λ l => let ds := parse_digits l.toList
+                                let d₁ := ds.head!
+                                let d₂ := ds.reverse.head!
+                                d₁ * 10 + d₂)
+  let sum := nums.sum
+  IO.println s!"values are {nums}"
+  IO.println s!"Their sum is {sum}"
+
+def main : IO Unit := sum_by List.parse_digits'
