2023/P02.lean
@@ -1,0 +1,70 @@
+import Lib
+
+abbrev CubeSet := ℕ
+
+abbrev Color := ℕ
+abbrev Color.red := 2
+abbrev Color.green := 3
+abbrev Color.blue := 5
+
+abbrev cube_set (counts : List (Color × ℕ)) : CubeSet := counts.prod_by (λ ⟨color, count⟩ => color ^ count)
+
+abbrev bag : CubeSet := cube_set [(.red, 12), (.green, 13), (.blue, 14)]
+
+structure Game where
+  id : ℕ
+  sets : List CubeSet
+deriving Inhabited
+
+instance : ToString Game where
+  toString | ⟨id, _⟩ => ToString.toString id
+
+def Game.is_possible (g : Game) (s : CubeSet) : Bool := g.sets.all (s % · == 0)
+
+def Game.parse (l : String) : Game :=
+  let parse_color : String → Color
+      | "red" => .red
+      | "green" => .green
+      | "blue" => .blue
+      | s => panic s!"invalid color {s}"
+  let parse_count (str : String) : (Color × ℕ) := match str.trim.splitOn " " with
+      | [count, color] => (parse_color color, count.toNat!)
+      | _ => panic s!"invalid count string {str}"
+  let parse_cube_set (str : String) : CubeSet := cube_set $ (str.trim.splitOn ",").map parse_count
+  match l.splitOn ":" with
+  | [game, rest] =>
+    match game.trim.splitOn " " with
+    | [_, id] => Game.mk id.toNat! (rest |>.splitOn ";"
+                                         |>.map parse_cube_set)
+    | _ => panic "invalid"
+  | _ => panic "invalid"
+
+partial
+
+
+def CubeSet.power (s : CubeSet) : ℕ :=
+  -- poor life choice lol
+  let rec count_color (s : CubeSet) (color : Color) : ℕ :=
+    if s % color == 0 then 1 + (count_color (s / color) color) else 0
+  [.red, .green, .blue].prod_by (count_color s ·)
+
+def read_games : IO (List Game) := do
+  let lines ← (← IO.getStdin).lines
+  return lines.map Game.parse
+
+def q1 : IO Unit := do
+  let games ← read_games
+  let valid_games := games.filter (·.is_possible bag)
+  let id_sum := (valid_games.map Game.id).sum
+  IO.println s!"Valid games are {valid_games}"
+  IO.println s!"Their sum is {id_sum}"
+
+def q2 : IO Unit := do
+  let lcm (n₁ n₂ : ℕ) : ℕ := n₁ * n₂ / n₁.gcd n₂
+  let games ← read_games
+  let powers := games.map (λ g => CubeSet.power (g.sets.foldl lcm 1))
+  let sum := powers.sum
+  IO.println s!"The powers are {powers}"
+  IO.println s!"Their sum is {sum}"
+
+def main : IO Unit := q1
