2023/lakefile.lean
@@ -9,3 +9,7 @@ lean_lib Lib
 @[default_target]
 lean_exe P01 where
   root := `P01
+
+@[default_target]
+lean_exe P02 where
+  root := `P02
